VL Updates...
 - Added basic support for tasks.  This involves the usual: a new
   vl-taskdecl-p structure for representing tasks, parsing and printing
   support, and various updates throughout mlib for functions like allexprs.
   There's no support for modeling/translating/synthesizing tasks, but this is
   at least good enough to see them and know they're in the namespace, etc.

 - Fix printing bug with case statements not printing a newline, which could
   cause malformed output like "endcaseend" instead of "endcase[\n]end".

 - Fix printing bug with enable statements that have no arguments.  They must
   print as, e.g., foo, instead of foo().

 - Fix printing bug with system function calls that have no arguments.  They
   must print as, e.g., $realtime, instead of $realtime().

 - Make argresolve more permissive.  In particular, it was previously a fatal
   warning to leave out ports when using named connections to a module, e.g.,
   if you had a module like:

      module adder (sum, a, b, cin);

   And tried to instance it like this;

      adder myadder (.sum(s), .a(abus), .b(bbus));

   Then argresolve would issue a fatal warning since cin is missing.  It turns
   out that other Verilog tools accept this bad syntax, treating it as though
   you had written:

      adder myadder (.sum(s), .a(abus), .b(bbus), .cin());

   So, for better compatibility with these tools, we now only treat the
   missing ports as unconnected, and issue only a non-fatal warning.

 - Add a basic way to limit the assignment-propagation transform to simple
   assignments, to prevent it from creating giant, unreadable expressions.

 - Extend the inlining transform to be able to handle blank arguments.

books/xdoc-impl/import-acl2doc.lisp
@@ -117,7 +117,24 @@ PL: ~pl[test-broken-link]~/~/")
 
 #!XDOC
 ;; Actually install the ground-zero topics
-(table xdoc 'doc (append *acl2-ground-zero-topics* (get-xdoc-table world)))
+(table xdoc 'doc
+
+; Something subtle about this is, what do we do if there is both an ACL2 :doc
+; topic and an XDOC topic?
+;
+; Originally we appended the *acl2-ground-zero-topics* to (get-xdoc-table
+; world), which meant that built-in ACL2 documentation "won" and overwrote the
+; xdoc documentation.  But when I documented the system/io.lisp book, I found
+; that this wasn't what I wanted, because it meant stupid tiny little
+; placeholder documentation for things like read-char$ was overwriting the much
+; nicer XDOC documentation for it.
+;
+; Arguably we should do some kind of smart merge, but, well, this *is* xdoc
+; after all.  So I'm just going to say ACL2 loses, and if someone cares enough
+; to come up with something better, power to them.
+
+       (append (get-xdoc-table world)
+               *acl2-ground-zero-topics*))
 
 (defxdoc acl2
   :short "Documentation for the <a
