books/centaur/vl/loader/parse-functions.lisp
@@ -25,21 +25,23 @@
 (local (include-book "../util/arithmetic"))
 
 
-; function_range_or_type ::= ['signed'] range
-;                          | 'integer'
-;                          | 'real'
-;                          | 'realtime'
-;                          | 'time'
+; function_range_or_type ::= ['signed'] range | 'integer' | 'real' | 'realtime' | 'time'
 
 (defparser vl-parse-optional-function-range-or-type (tokens warnings)
   :result (and (consp val)
-               (vl-funtype-p (car val))
+               (vl-taskporttype-p (car val))
                (vl-maybe-range-p (cdr val)))
   :fails gracefully
   :count weak
   (seqw tokens warnings
-        (when (vl-is-some-token? '(:vl-kwd-integer :vl-kwd-real :vl-kwd-realtime :vl-kwd-time))
-          (vartype-token := (vl-match-some-token '(:vl-kwd-integer :vl-kwd-real :vl-kwd-realtime :vl-kwd-time)))
+        (when (vl-is-some-token? '(:vl-kwd-integer
+                                   :vl-kwd-real
+                                   :vl-kwd-realtime
+                                   :vl-kwd-time))
+          (vartype-token := (vl-match-some-token '(:vl-kwd-integer
+                                                   :vl-kwd-real
+                                                   :vl-kwd-realtime
+                                                   :vl-kwd-time)))
           (return (cons (case (vl-token->type vartype-token)
                           (:vl-kwd-integer  :vl-integer)
                           (:vl-kwd-real     :vl-real)
@@ -53,202 +55,230 @@
         (return (cons (if signed :vl-signed :vl-unsigned) range))))
 
 
-
 ; tf_input_declaration ::= 'input' [ 'reg' ] [ 'signed' ] [ range ] list_of_port_identifiers
+;                        | 'input' task_port_type list_of_port_identifiers
+;
+; tf_output_declaration ::= 'output' [ 'reg' ] [ 'signed' ] [ range ] list_of_port_identifiers
+;                        | 'input' task_port_type list_of_port_identifiers
+;
+; tf_inout_declaration ::= 'inout' [ 'reg' ] [ 'signed' ] [ range ] list_of_port_identifiers
 ;                        | 'input' task_port_type list_of_port_identifiers
 ;
 ; task_port_type ::= 'integer' | 'real' | 'realtime' | 'time'
 ;
 ; list_of_port_identifier ::= identifier { ',' identifier }
 
-(defsection vl-build-function-inputs
+(defsection vl-build-taskports
 
-  (defund vl-build-function-inputs (atts type range names)
+  (defund vl-build-taskports (atts dir type range names)
     (declare (xargs :guard (and (vl-atts-p atts)
-                                (vl-funtype-p type)
+                                (vl-direction-p dir)
+                                (vl-taskporttype-p type)
                                 (vl-maybe-range-p range)
                                 (vl-idtoken-list-p names))))
     (if (atom names)
         nil
-      (cons (make-vl-funinput :name  (vl-idtoken->name (car names))
+      (cons (make-vl-taskport :name  (vl-idtoken->name (car names))
+                              :dir   dir
                               :type  type
                               :range range
                               :atts  atts
                               :loc   (vl-token->loc (car names)))
-            (vl-build-function-inputs atts type range (cdr names)))))
+            (vl-build-taskports atts dir type range (cdr names)))))
 
-  (local (in-theory (enable vl-build-function-inputs)))
+  (local (in-theory (enable vl-build-taskports)))
 
-  (defthm vl-funinputlist-p-of-vl-build-function-inputs
+  (defthm vl-taskportlist-p-of-vl-build-taskports
     (implies (and (force (vl-atts-p atts))
-                  (force (vl-funtype-p type))
+                  (force (vl-direction-p dir))
+                  (force (vl-taskporttype-p type))
                   (force (vl-maybe-range-p range))
                   (force (vl-idtoken-list-p names)))
-             (vl-funinputlist-p (vl-build-function-inputs atts type range names)))))
+             (vl-taskportlist-p (vl-build-taskports atts dir type range names)))))
 
-
-(defparser vl-parse-function-input-declaration (atts tokens warnings)
-  ;; Matches tf_input_declaration, for functions.
+(defparser vl-parse-taskport-declaration (atts tokens warnings)
+  ;; Matches tf_input_declaration, tf_output_declaration, or tf_inout_declaration.
   :guard (vl-atts-p atts)
-  :result (vl-funinputlist-p val)
+  :result (vl-taskportlist-p val)
   :resultp-of-nil t
   :true-listp t
   :fails gracefully
   :count strong
   (seqw tokens warnings
-        (:= (vl-match-token :vl-kwd-input))
+        (dir := (vl-match-some-token '(:vl-kwd-input :vl-kwd-output :vl-kwd-inout)))
         (when (vl-is-token? :vl-kwd-reg)
           (reg := (vl-match-token :vl-kwd-reg)))
         (when (vl-is-token? :vl-kwd-signed)
           (signed := (vl-match-token :vl-kwd-signed)))
         (when (vl-is-token? :vl-lbrack)
           (range := (vl-parse-range)))
-        (when (vl-is-some-token? '(:vl-kwd-integer :vl-kwd-real :vl-kwd-realtime :vl-kwd-time))
-          (type := (vl-match-some-token '(:vl-kwd-integer :vl-kwd-real :vl-kwd-realtime :vl-kwd-time))))
+        (when (vl-is-some-token? '(:vl-kwd-integer
+                                   :vl-kwd-real
+                                   :vl-kwd-realtime
+                                   :vl-kwd-time))
+          (type := (vl-match-some-token '(:vl-kwd-integer
+                                          :vl-kwd-real
+                                          :vl-kwd-realtime
+                                          :vl-kwd-time))))
         (names := (vl-parse-1+-identifiers-separated-by-commas))
         (return-raw
-         (if (and type (or reg signed range))
-             (vl-parse-error "Function input declarations cannot have ~
-                              variable types with reg/signed keywords or ~
-                              ranges.")
-           (let ((ret (vl-build-function-inputs
-                       atts
-                       (case type
-                         (:vl-kwd-integer  :vl-integer)
-                         (:vl-kwd-real     :vl-real)
-                         (:vl-kwd-realtime :vl-realtime)
-                         (:vl-kwd-time     :vl-time)
-                         (otherwise
-                          ;; BOZO Question: does the reg keyword actually do
-                          ;; anything?  I think the answer is "no."  I haven't
-                          ;; been able to see a difference resulting from
-                          ;; saying "input reg v" versus "input v" for
-                          ;; functions.  But But I have no justification for
-                          ;; this.  A quick internet search revealed nothing.
-                          ;; I don't know who would know what the answer is.
-                          (if signed
-                              :vl-signed
-                            :vl-unsigned)))
-                       range names)))
-             (mv nil ret tokens warnings))))))
+         (b* (((when (and type (or reg signed range)))
+               (vl-parse-error "Task/function port declarations cannot ~
+                                combine reg/signed keyword with variable ~
+                                types (integer, real, realtime, time)."))
+              (dir (case (vl-token->type dir)
+                     (:vl-kwd-input    :vl-input)
+                     (:vl-kwd-output   :vl-output)
+                     (:vl-kwd-inout    :vl-inout)))
+              (type (if type
+                        (case (vl-token->type type)
+                          (:vl-kwd-integer  :vl-integer)
+                          (:vl-kwd-real     :vl-real)
+                          (:vl-kwd-realtime :vl-realtime)
+                          (:vl-kwd-time     :vl-time))
+                      (if signed
+                          :vl-signed
+                        :vl-unsigned)))
+              (ret (vl-build-taskports atts dir type range names)))
+           (mv nil ret tokens warnings)))))
 
 
-
+; task_port_item ::= { attribute_instance } tf_input_declaration
+;                  | { attribute_instance } tf_output_declaration
+;                  | { attribute_instance } tf_inout_declaration
+;
+; task_port_list ::= task_port_item { , task_port_item }
+;
 ; function_port_list ::= { attribute_instance } tf_input_declaration
-;                              { ',' { attribute_instance } tf_input_declaration }
+;                          { ',' { attribute_instance } tf_input_declaration }
+;
+; Note: function_port_list is just the subset of task_port_list where the ports
+; are all of type input.
+;
+; Our approach: just write a parser for task_port_list, then separately check
+; (when we construct the function declaration) that all the ports are inputs.
 
-(defparser vl-parse-function-port-list (tokens warnings)
-  :result (vl-funinputlist-p val)
+(defparser vl-parse-taskport-list (tokens warnings)
+  :result (vl-taskportlist-p val)
   :resultp-of-nil t
   :true-listp t
   :fails gracefully
   :count strong
   (seqw tokens warnings
         (atts := (vl-parse-0+-attribute-instances))
-        (ins1 := (vl-parse-function-input-declaration atts))
+        (ins1 := (vl-parse-taskport-declaration atts))
         (unless (vl-is-token? :vl-comma)
           (return ins1))
         (:= (vl-match-token :vl-comma))
-        (ins2 := (vl-parse-function-port-list))
+        (ins2 := (vl-parse-taskport-list))
         (return (append ins1 ins2))))
 
 
+; task_item_declaration ::= block_item_declaration
+;                         | { attribute_instance } tf_input_declaration ';'
+;                         | { attribute_instance } tf_output_declaration ';'
+;                         | { attribute_instance } tf_inout_declaration ';'
+;
 ; function_item_declaration ::= block_item_declaration
 ;                             | { attribute_instance } tf_input_declaration ';'
+;
+; Note: again, function_item_declaration is the subset of task_item_declaration
+; where the only ports are inputs.
+;
+; Our approach: just writer a parser for task_item_declaration, then separately
+; check (when we construct the function declaration) that all ports are inputs.
 
-(defsection vl-funinput-or-blockitem-p
+(defsection vl-taskport-or-blockitem-p
 
-  (defund vl-funinput-or-blockitem-p (x)
+  (defund vl-taskport-or-blockitem-p (x)
     (declare (xargs :guard t))
-    (or (vl-funinput-p x)
+    (or (vl-taskport-p x)
         (vl-blockitem-p x)))
 
-  (deflist vl-funinput-or-blockitem-list-p (x)
-    (vl-funinput-or-blockitem-p x)
+  (deflist vl-taskport-or-blockitem-list-p (x)
+    (vl-taskport-or-blockitem-p x)
     :guard t
     :elementp-of-nil nil)
 
-  (local (in-theory (enable vl-funinput-or-blockitem-p)))
+  (local (in-theory (enable vl-taskport-or-blockitem-p)))
 
-  (defthm vl-funinput-or-blockitem-list-p-when-vl-funinputlist-p
-    (implies (vl-funinputlist-p x)
-             (vl-funinput-or-blockitem-list-p x))
+  (defthm vl-taskport-or-blockitem-list-p-when-vl-taskportlist-p
+    (implies (vl-taskportlist-p x)
+             (vl-taskport-or-blockitem-list-p x))
     :hints(("Goal" :induct (len x))))
 
-  (defthm vl-funinput-or-blockitem-list-p-when-vl-blockitemlist-p
+  (defthm vl-taskport-or-blockitem-list-p-when-vl-blockitemlist-p
     (implies (vl-blockitemlist-p x)
-             (vl-funinput-or-blockitem-list-p x))
+             (vl-taskport-or-blockitem-list-p x))
     :hints(("Goal" :induct (len x))))
 
   (local (defthm crock
-           (implies (vl-funinput-or-blockitem-p x)
-                    (equal (vl-funinput-p x)
-                           (eq (tag x) :vl-funinput)))
+           (implies (vl-taskport-or-blockitem-p x)
+                    (equal (vl-taskport-p x)
+                           (eq (tag x) :vl-taskport)))
            :hints(("Goal" :in-theory (enable vl-blockitem-p)))))
 
-  (defund vl-filter-funinput-or-blockitem-list (x)
-    (declare (xargs :guard (vl-funinput-or-blockitem-list-p x)))
+  (defund vl-filter-taskport-or-blockitem-list (x)
+    (declare (xargs :guard (vl-taskport-or-blockitem-list-p x)))
     (b* (((when (atom x))
           (mv nil nil))
-         ((mv cdr-funinputs cdr-blockitems)
-          (vl-filter-funinput-or-blockitem-list (cdr x))))
-      (if (eq (tag (car x)) :vl-funinput)
-          (mv (cons (car x) cdr-funinputs)
-              cdr-blockitems)
-        (mv cdr-funinputs (cons (car x) cdr-blockitems)))))
+         ((mv cdr-taskports cdr-blockitems)
+          (vl-filter-taskport-or-blockitem-list (cdr x)))
+         ((when (eq (tag (car x)) :vl-taskport))
+          (mv (cons (car x) cdr-taskports) cdr-blockitems)))
+      (mv cdr-taskports (cons (car x) cdr-blockitems))))
 
-  (defthm vl-filter-funinput-or-blockitem-list-basics
-    (implies (force (vl-funinput-or-blockitem-list-p x))
-             (let ((ret (vl-filter-funinput-or-blockitem-list x)))
-               (and (vl-funinputlist-p (mv-nth 0 ret))
+  (defthm vl-filter-taskport-or-blockitem-list-basics
+    (implies (force (vl-taskport-or-blockitem-list-p x))
+             (let ((ret (vl-filter-taskport-or-blockitem-list x)))
+               (and (vl-taskportlist-p (mv-nth 0 ret))
                     (vl-blockitemlist-p (mv-nth 1 ret)))))
-    :hints(("Goal" :in-theory (enable vl-filter-funinput-or-blockitem-list)))))
+    :hints(("Goal" :in-theory (enable vl-filter-taskport-or-blockitem-list)))))
 
 
-
-(defparser vl-parse-function-item-declaration-noatts (atts tokens warnings)
+(defparser vl-parse-task-item-declaration-noatts (atts tokens warnings)
   :guard (vl-atts-p atts)
-  :result (vl-funinput-or-blockitem-list-p val)
+  :result (vl-taskport-or-blockitem-list-p val)
   :true-listp t
   :resultp-of-nil t
   :fails gracefully
   :count strong
   (seqw tokens warnings
-        (when (vl-is-token? :vl-kwd-input)
-          (decls := (vl-parse-function-input-declaration atts tokens warnings))
+        (when (vl-is-some-token? '(:vl-kwd-input :vl-kwd-output :vl-kwd-inout))
+          (decls := (vl-parse-taskport-declaration atts tokens warnings))
           (:= (vl-match-token :vl-semi))
           (return decls))
         (decls := (vl-parse-block-item-declaration-noatts atts tokens warnings))
         (return decls)))
 
-(defparser vl-parse-function-item-declaration (tokens warnings)
-  :result (vl-funinput-or-blockitem-list-p val)
+(defparser vl-parse-task-item-declaration (tokens warnings)
+  :result (vl-taskport-or-blockitem-list-p val)
   :resultp-of-nil t
   :true-listp t
   :fails gracefully
   :count strong
   (seqw tokens warnings
-        (atts := (vl-parse-0+-attribute-instances))
-        (decls := (vl-parse-function-item-declaration-noatts atts))
+        (atts  := (vl-parse-0+-attribute-instances))
+        (decls := (vl-parse-task-item-declaration-noatts atts))
         (return decls)))
 
-(defparser vl-parse-0+-function-item-declarations (tokens warnings)
-  ;; Tries to eat as many function items as it can find.
+(defparser vl-parse-0+-task-item-declarations (tokens warnings)
+  ;; Tries to eat as many task items as it can find.
   ;; We use backtracking to know when to stop, because these declarations can be
   ;; followed by arbitrary statements, hence it's not clear whether (* ... *) is
-  ;; the start of a new block item declaration or a statement.
-  :result (vl-funinput-or-blockitem-list-p val)
+  ;; the start of a new item declaration or a statement.
+  :result (vl-taskport-or-blockitem-list-p val)
   :resultp-of-nil t
   :true-listp t
   :fails never
   :count strong-on-value
   (mv-let (erp first explore new-warnings)
-    (vl-parse-function-item-declaration)
+    (vl-parse-task-item-declaration)
     (cond (erp
            (mv nil nil tokens warnings))
           (t
            (mv-let (erp rest tokens warnings)
-             (vl-parse-0+-function-item-declarations explore new-warnings)
+             (vl-parse-0+-task-item-declarations explore new-warnings)
              (declare (ignore erp))
              (mv nil (append first rest) tokens warnings))))))
 
@@ -262,12 +292,32 @@
 ;      statement
 ;    'endfunction'
 ;
-;
 ;  | 'function' [ 'automatic' ] [ function_range_or_type ]              ; variant 2
 ;     identifier '(' function_port_list ')' ';'
 ;     { block_item_declaration }
 ;     statement
 ;    'endfunction'
+
+(defsection vl-taskportlist-find-noninput
+
+  (defund vl-taskportlist-find-noninput (x)
+    (declare (xargs :guard (vl-taskportlist-p x)))
+    (cond ((atom x)
+           nil)
+          ((eq (vl-taskport->dir (car x)) :vl-input)
+           (vl-taskportlist-find-noninput (cdr x)))
+          (t
+           (car x))))
+
+  (local (in-theory (enable vl-taskportlist-find-noninput)))
+
+  (defthm vl-taskport-p-of-vl-taskportlist-find-noninput
+    (implies (force (vl-taskportlist-p x))
+             (equal (vl-taskport-p (vl-taskportlist-find-noninput x))
+                    (if (vl-taskportlist-find-noninput x)
+                        t
+                      nil)))))
+
 
 (defparser vl-parse-function-declaration (atts tokens warnings)
   ;; Returns a (singleton) list of function decls instead of a just a function
@@ -289,19 +339,25 @@
         (when (vl-is-token? :vl-semi)
           ;; Variant 1.
           (:= (vl-match-token :vl-semi))
-          (decls := (vl-parse-0+-function-item-declarations))
+          (decls := (vl-parse-0+-task-item-declarations))
           (stmt := (vl-parse-statement))
           (:= (vl-match-token :vl-kwd-endfunction))
           (return-raw
-           (b* (((mv funinputs blockitems)
-                 (vl-filter-funinput-or-blockitem-list decls))
-                ((unless (consp funinputs))
+           (b* (((mv inputs blockitems)
+                 (vl-filter-taskport-or-blockitem-list decls))
+                (non-input (vl-taskportlist-find-noninput inputs))
+                ((when non-input)
+                 (vl-parse-error (str::cat "Functions may only have inputs, but port "
+                                           (vl-taskport->name non-input)
+                                           " has direction "
+                                           (symbol-name (vl-taskport->dir non-input)))))
+                ((unless (consp inputs))
                  (vl-parse-error "Function has no inputs."))
                 (ret (make-vl-fundecl :name       (vl-idtoken->name name)
                                       :automaticp (if automatic t nil)
                                       :rtype      rtype
                                       :rrange     rrange
-                                      :inputs     funinputs
+                                      :inputs     inputs
                                       :decls      blockitems
                                       :body       stmt
                                       :atts       atts
@@ -310,20 +366,272 @@
 
         ;; Variant 2.
         (:= (vl-match-token :vl-lparen))
-        (funinputs := (vl-parse-function-port-list))
+        (inputs := (vl-parse-taskport-list))
         (:= (vl-match-token :vl-rparen))
         (:= (vl-match-token :vl-semi))
         (blockitems := (vl-parse-0+-block-item-declarations))
         (stmt := (vl-parse-statement))
         (:= (vl-match-token :vl-kwd-endfunction))
-        (return
-         (list (make-vl-fundecl :name       (vl-idtoken->name name)
-                                :automaticp (if automatic t nil)
-                                :rtype      rtype
-                                :rrange     rrange
-                                :inputs     funinputs
-                                :decls      blockitems
-                                :body       stmt
-                                :atts       atts
-                                :loc        (vl-token->loc function))))))
+        (return-raw
+         (b* ((non-input (vl-taskportlist-find-noninput inputs))
+              ((when non-input)
+               (vl-parse-error (str::cat "Functions may only have inputs, but port "
+                                         (vl-taskport->name non-input)
+                                         " has direction "
+                                         (symbol-name (vl-taskport->dir non-input)))))
+              ;; (consp inputs) is automatic from vl-parse-taskport-list.
+              (ret (make-vl-fundecl :name       (vl-idtoken->name name)
+                                    :automaticp (if automatic t nil)
+                                    :rtype      rtype
+                                    :rrange     rrange
+                                    :inputs     inputs
+                                    :decls      blockitems
+                                    :body       stmt
+                                    :atts       atts
+                                    :loc        (vl-token->loc function))))
+           (mv nil (list ret) tokens warnings)))))
 
+
+
+
+; task_declaration ::=
+;
+;    'task' [ 'automatic' ] identifier ';'         ;; variant 1
+;       { task_item_declaration }
+;       statement_or_null
+;    'endtask'
+;
+;  | 'task' [ 'automatic' ] identifier '(' [task_port_list] ')' ';'
+;       { block_item_declaration }
+;       statement_or_null
+;    'endtask'
+
+(defparser vl-parse-task-declaration (atts tokens warnings)
+  ;; Returns a (singleton) list of task decls instead of a just a task
+  ;; declaration, to fit nicely into vl-parse-module-or-generate-item.
+  :guard (vl-atts-p atts)
+  :result (vl-taskdecllist-p val)
+  :true-listp t
+  :resultp-of-nil t
+  :fails gracefully
+  :count strong
+  (seqw tokens warnings
+
+        (task := (vl-match-token :vl-kwd-task))
+        (when (vl-is-token? :vl-kwd-automatic)
+          (automatic := (vl-match-token :vl-kwd-automatic)))
+        (name := (vl-match-token :vl-idtoken))
+
+        (when (vl-is-token? :vl-semi)
+          ;; Variant 1.
+          (:= (vl-match-token :vl-semi))
+          (decls := (vl-parse-0+-task-item-declarations))
+          (stmt  := (vl-parse-statement-or-null))
+          (:= (vl-match-token :vl-kwd-endtask))
+          (return
+           (b* (((mv ports blockitems)
+                 (vl-filter-taskport-or-blockitem-list decls)))
+             (list (make-vl-taskdecl :name       (vl-idtoken->name name)
+                                     :automaticp (if automatic t nil)
+                                     :ports      ports
+                                     :decls      blockitems
+                                     :body       stmt
+                                     :atts       atts
+                                     :loc        (vl-token->loc task))))))
+
+        ;; Variant 2.
+        (:= (vl-match-token :vl-lparen))
+        (ports := (vl-parse-taskport-list))
+        (:= (vl-match-token :vl-rparen))
+        (:= (vl-match-token :vl-semi))
+        (blockitems := (vl-parse-0+-block-item-declarations))
+        (stmt       := (vl-parse-statement-or-null))
+        (:= (vl-match-token :vl-kwd-endtask))
+        (return (list (make-vl-taskdecl :name       (vl-idtoken->name name)
+                                        :automaticp (if automatic t nil)
+                                        :ports      ports
+                                        :decls      blockitems
+                                        :body       stmt
+                                        :atts       atts
+                                        :loc        (vl-token->loc task))))))
+
+
+(local
+ (encapsulate
+   ()
+
+   (local (include-book "lexer")) ;; for making test inputs from strings
+
+   (defund taskport-summary (x)
+     (declare (xargs :guard (vl-taskport-p x)))
+     (b* (((vl-taskport x) x))
+       (list x.name x.dir x.type (vl-pretty-maybe-range x.range))))
+
+   (defprojection taskportlist-summary (x)
+     (taskport-summary x)
+     :guard (vl-taskportlist-p x))
+
+   (defmacro test-parse-taskports (&key input (successp 't) summary)
+     `(with-output
+        :off summary
+        (assert! (b* (((mv erp val tokens warnings)
+                       (vl-parse-taskport-list (vl-make-test-tstream ,input)
+                                               'blah-warnings))
+
+                      ((unless ,successp)
+                       (cw "Expected failure.~%")
+                       (cw "Actual erp: ~x0.~%" erp)
+                       erp)
+
+                      ((when erp)
+                       (cw "Expected success, but ERP is ~x0~%" erp))
+
+                      (spec-summary ',summary)
+                      (impl-summary (taskportlist-summary val)))
+                   (and (progn$
+                         (cw "Spec-Summary: ~x0~%" spec-summary)
+                         (cw "Impl-Summary: ~x0~%" impl-summary)
+                         (equal spec-summary impl-summary))
+                        (progn$
+                         (cw "Tokens: ~x0~%" tokens)
+                         (not tokens))
+                        (progn$
+                         (cw "Warnings: ~x0~%" warnings)
+                         (equal warnings 'blah-warnings)))))))
+
+
+   (test-parse-taskports :input ""
+                         :successp nil)
+
+   (test-parse-taskports :input "foo"
+                         :successp nil)
+
+   (test-parse-taskports :input "input a"
+                         :summary (("a" :vl-input :vl-unsigned (no-range))))
+
+   (test-parse-taskports :input "input a, b"
+                         :summary (("a" :vl-input :vl-unsigned (no-range))
+                                   ("b" :vl-input :vl-unsigned (no-range))))
+
+   (test-parse-taskports :input "input a, b, c, d"
+                         :summary (("a" :vl-input :vl-unsigned (no-range))
+                                   ("b" :vl-input :vl-unsigned (no-range))
+                                   ("c" :vl-input :vl-unsigned (no-range))
+                                   ("d" :vl-input :vl-unsigned (no-range))))
+
+;; bozo we're currently ignoring reg.  does it mean anything?
+   (test-parse-taskports :input "input reg a"
+                         :summary (("a" :vl-input :vl-unsigned (no-range))))
+
+   (test-parse-taskports :input "input reg a, b"
+                         :summary (("a" :vl-input :vl-unsigned (no-range))
+                                   ("b" :vl-input :vl-unsigned (no-range))))
+
+   (test-parse-taskports :input "input signed a"
+                         :summary (("a" :vl-input :vl-signed (no-range))))
+
+   (test-parse-taskports :input "input signed a, b"
+                         :summary (("a" :vl-input :vl-signed (no-range))
+                                   ("b" :vl-input :vl-signed (no-range))))
+
+
+   (test-parse-taskports :input "input [3:0] a"
+                         :summary (("a" :vl-input :vl-unsigned (range 3 0))))
+
+   (test-parse-taskports :input "input [3:0] a, b"
+                         :summary (("a" :vl-input :vl-unsigned (range 3 0))
+                                   ("b" :vl-input :vl-unsigned (range 3 0))))
+
+   (test-parse-taskports :input "input [3:0] a, b, \c , d"
+                         :summary (("a" :vl-input :vl-unsigned (range 3 0))
+                                   ("b" :vl-input :vl-unsigned (range 3 0))
+                                   ("c" :vl-input :vl-unsigned (range 3 0))
+                                   ("d" :vl-input :vl-unsigned (range 3 0))
+                                   ))
+
+   (test-parse-taskports :input "input signed [3:0] a"
+                         :summary (("a" :vl-input :vl-signed (range 3 0))))
+
+   (test-parse-taskports :input "input signed [3:0] a, b"
+                         :summary (("a" :vl-input :vl-signed (range 3 0))
+                                   ("b" :vl-input :vl-signed (range 3 0))))
+
+   (test-parse-taskports :input "input reg [3:0] a"
+                         :summary (("a" :vl-input :vl-unsigned (range 3 0))))
+
+   (test-parse-taskports :input "input reg signed [3:0] a"
+                         :summary (("a" :vl-input :vl-signed (range 3 0))))
+
+   (test-parse-taskports :input "input integer a"
+                         :summary (("a" :vl-input :vl-integer (no-range))))
+
+   (test-parse-taskports :input "input real a"
+                         :summary (("a" :vl-input :vl-real (no-range))))
+
+   (test-parse-taskports :input "input time a"
+                         :summary (("a" :vl-input :vl-time (no-range))))
+
+   (test-parse-taskports :input "input realtime a"
+                         :summary (("a" :vl-input :vl-realtime (no-range))))
+
+
+;; reg must come before signed
+   (test-parse-taskports :input "input signed reg a"
+                         :successp nil)
+
+;; signed not okay with int/real/time/realtime
+   (test-parse-taskports :input "input integer signed a" :successp nil)
+   (test-parse-taskports :input "input signed integer a" :successp nil)
+   (test-parse-taskports :input "input real signed a" :successp nil)
+   (test-parse-taskports :input "input signed real a" :successp nil)
+   (test-parse-taskports :input "input integer signed a" :successp nil)
+   (test-parse-taskports :input "input signed integer a" :successp nil)
+   (test-parse-taskports :input "input integer signed a" :successp nil)
+   (test-parse-taskports :input "input signed integer a" :successp nil)
+   (test-parse-taskports :input "input time signed a" :successp nil)
+   (test-parse-taskports :input "input signed time a" :successp nil)
+   (test-parse-taskports :input "input time signed a" :successp nil)
+   (test-parse-taskports :input "input signed time a" :successp nil)
+   (test-parse-taskports :input "input realtime signed a" :successp nil)
+   (test-parse-taskports :input "input signed realtime a" :successp nil)
+   (test-parse-taskports :input "input realtime signed a" :successp nil)
+   (test-parse-taskports :input "input signed realtime a" :successp nil)
+
+;; reg not okay with int/real/time/realtime
+   (test-parse-taskports :input "input integer reg a" :successp nil)
+   (test-parse-taskports :input "input reg integer a" :successp nil)
+   (test-parse-taskports :input "input real reg a" :successp nil)
+   (test-parse-taskports :input "input reg real a" :successp nil)
+   (test-parse-taskports :input "input integer reg a" :successp nil)
+   (test-parse-taskports :input "input reg integer a" :successp nil)
+   (test-parse-taskports :input "input integer reg a" :successp nil)
+   (test-parse-taskports :input "input reg integer a" :successp nil)
+   (test-parse-taskports :input "input time reg a" :successp nil)
+   (test-parse-taskports :input "input reg time a" :successp nil)
+   (test-parse-taskports :input "input time reg a" :successp nil)
+   (test-parse-taskports :input "input reg time a" :successp nil)
+   (test-parse-taskports :input "input realtime reg a" :successp nil)
+   (test-parse-taskports :input "input reg realtime a" :successp nil)
+   (test-parse-taskports :input "input realtime reg a" :successp nil)
+   (test-parse-taskports :input "input reg realtime a" :successp nil)
+
+;; range not okay with int/real/time/realtime
+   (test-parse-taskports :input "input integer [3:0] a" :successp nil)
+   (test-parse-taskports :input "input [3:0] integer a" :successp nil)
+   (test-parse-taskports :input "input real [3:0] a" :successp nil)
+   (test-parse-taskports :input "input [3:0] real a" :successp nil)
+   (test-parse-taskports :input "input integer [3:0] a" :successp nil)
+   (test-parse-taskports :input "input [3:0] integer a" :successp nil)
+   (test-parse-taskports :input "input integer [3:0] a" :successp nil)
+   (test-parse-taskports :input "input [3:0] integer a" :successp nil)
+   (test-parse-taskports :input "input time [3:0] a" :successp nil)
+   (test-parse-taskports :input "input [3:0] time a" :successp nil)
+   (test-parse-taskports :input "input time [3:0] a" :successp nil)
+   (test-parse-taskports :input "input [3:0] time a" :successp nil)
+   (test-parse-taskports :input "input realtime [3:0] a" :successp nil)
+   (test-parse-taskports :input "input [3:0] realtime a" :successp nil)
+   (test-parse-taskports :input "input realtime [3:0] a" :successp nil)
+   (test-parse-taskports :input "input [3:0] realtime a" :successp nil)
+
+
+   ))
